Tests/EvmSdkSpec.lean
@@ -43,6 +43,7 @@ def fungibleAllowances : Fungible.Allowances := secondMap.handle
 #guard SafeErc20.transfer paymentAddress paymentAddress paymentAmount == 9
 #guard SafeErc20.approve paymentAddress paymentAddress paymentAmount == 9
 #guard SafeErc20.transferFrom paymentAddress paymentAddress paymentAddress paymentAmount == 9
+#guard SafeErc20.forceApprove paymentAddress paymentAddress paymentAmount == 9
 #guard Erc2981.feeDenominator == ⟨10000, 0, 0, 0⟩
 #guard Erc165.erc2981 == ⟨0x5a20552a, 0, 0, 0⟩
 #guard WETH.deposit paymentAddress paymentAmount == 9
